Inductive Hypothesis
T(n) = n lgn

Base Case
If n = 2, then T(n) = 2. n * lgn becomes 2 * lg2 = 2.

Inductive Step
Suppose that for some value l in the natural numbers if k = 2^l then T(k) = k lgk.
We want to prove that for l + 1, T(k) = k lgk.
k = 2^l * 2

T(2^l) = 2T(2^l-1) + 2^(l-1) * 2 = 2^l * lg(2^l)

T(2^l * 2) = 2T((2^l * 2)/2) + 2^l * 2
                  = 2T(2^l) + 2^l * 2
                  = 2(2^l * lg(2^l)) + 2^l * 2
                  = (2^l + 1) * lg(2^l) + 2^(l + 1)
                  = k * lg(2^l) + k
                  = k * (lg(2^l * 2 / 2)) + k
                  = k * (lg(k / 2)) + k
                  = k * (lg(k) - 1) + k
                  = klgk